DY/Misc.lean
@@ -12,3 +12,37 @@ instance: Std.OrientedOrd Unit where
 
 instance: Std.TransOrd Unit where
   isLE_trans := by grind
+
+def ByteArray.compare (x y: ByteArray): Ordering :=
+  Ord.compare x.data y.data
+
+instance: Ord ByteArray where
+  compare x y := ByteArray.compare x y
+
+instance: Std.ReflOrd ByteArray where
+  compare_self := by
+    simp only [compare]
+    simp [ByteArray.compare]
+
+instance: Std.LawfulEqOrd ByteArray where
+  eq_of_compare := by
+    simp only [compare]
+    simp only [ByteArray.compare]
+    intro ⟨ x ⟩ ⟨ y ⟩ h
+    simp only [ByteArray.mk.injEq]
+    apply Std.LawfulEqOrd.eq_of_compare
+    exact h
+
+instance: Std.OrientedOrd ByteArray where
+  eq_swap := by
+    simp only [compare]
+    simp only [ByteArray.compare]
+    intro x y
+    apply Std.OrientedOrd.eq_swap
+
+instance: Std.TransOrd ByteArray where
+  isLE_trans := by
+    simp only [compare]
+    simp only [ByteArray.compare]
+    intro x y z
+    apply Std.TransOrd.isLE_trans
